confusing error

src/lib/poly/gemm/Kuiper.Poly.GEMM.TensorCore2D.fst
@@ -13,6 +13,7 @@ open Kuiper.Math { even, odd, even_2x, odd_2x1 }
 open Kuiper.Matrix
 
 module MS = Kuiper.Spec.GEMM
+module T = FStar.Tactics.V2
 module SZ = FStar.SizeT
 module B = Kuiper.Barrier
 
@@ -32,6 +33,7 @@ open Kuiper.Poly.GEMM.Copy
 open Kuiper.Poly.GEMM.Tiled.Common
 
 open Pulse.Lib.Array
+open Pulse.Lib.Trade
 
 let array_fragment_pts_to
   (#et : Type0)
@@ -39,32 +41,71 @@ let array_fragment_pts_to
   (#m #n #k : nat)
   (#l : fragment_layout)
   ([@@@mkey] farr: array (fragment et knd m n k l))
+  (#[T.exact (`1.0R)] f : perm)
   (ems : seq (value_for et knd m n k))
   : slprop = 
-    exists* (s: lseq (fragment et knd m n k l) (len ems)).
-      farr |-> s **
-      forall+ (i : natlt (Seq.length s)).
-        (s @! i) |-> (ems @! i)
+    exists* (s: lseq (fragment et knd m n k l) (Seq.length ems)).
+      farr |-> Frac f s **
+      forall+ (i : natlt (Seq.length ems)).
+        (s @! i) |-> Frac f (ems @! i)
 
 ghost
-fn gpu_array_fragment_extract
+fn array_fragment_extract
   (#et:Type0)
   (#knd : fragment_kind)
   (#m #n #k : nat)
   (#l : fragment_layout)
-  ([@@@mkey] farr: array (fragment et knd m n k l))
-  (ems : seq (value_for et knd m n k))
-  (i : natlt (len ems))
-  (#em : (let o, p = (dims_for knd m n k) in ematrix et o p))
+  (farr: array (fragment et knd m n k l))
+  // without erased despite ghost fn, there are too many reveals when used
+  // In this implementation probably due to loop invariants?
+  (ems : erased (seq (value_for et knd m n k)))
   (#f : perm)
+  (i : natlt (Seq.length ems))
+  ()
   requires
-    array_fragment_pts_to 
-  ensures
-    factored
-      (gpu_matrix_subtile gm trows tcols tr tc |-> Frac f (ematrix_subtile em trows tcols tr tc))
-      (gm |-> Frac f em)
+    array_fragment_pts_to farr #f ems
+  // ensures
+  //   exists* (s : (lseq (fragment et knd m n k l) (Seq.length ems))).
+  //     farr |-> Frac f s **
+  //     (s @! i) |-> Frac f (ems @! i) **
+  //     (forall* (em' : value_for et knd m n k).
+  //       farr |-> Frac f s **
+  //        (s @! i) |-> Frac f em' @==>
+  //         array_fragment_pts_to farr #f (Seq.upd ems i em'))
+{
+  unfold array_fragment_pts_to;
+  // Why "cannot find typeclass"?
+  // with s. assert farr |-> Frac f s;
+  with s. assert pts_to farr #f s;
 
+  forevery_extract' i (fun (x : natlt (len s)) -> (s @! x) |-> (ems @! x));
+  admit();
+}
 
+// ghost
+// fn array_fragment_extract_ro
+//   (#et:Type0)
+//   (#knd : fragment_kind)
+//   (#m #n #k : nat)
+//   (#l : fragment_layout)
+//   (farr: array (fragment et knd m n k l))
+//   (ems : seq (value_for et knd m n k))
+//   (i : natlt (len ems))
+//   // (#em : (let o, p = (dims_for knd m n k) in ematrix et o p))
+//   (#f : perm)
+//   (#s: lseq (fragment et knd m n k l) (len ems))
+//   requires
+//     farr |-> Frac f s **
+//     (forall+ (i : natlt (Seq.length s)). (s @! i) |-> Frac f (ems @! i))
+//   ensures
+//     factored
+//       ((s @! i) |-> Frac f (ems @! i))
+//       (farr |-> s **
+//        (forall+ (i : natlt (Seq.length s)). (s @! i) |-> Frac f (ems @! i)))
+
+// {
+//   admit();
+// }
 
 // inline_for_extraction noextract
 // fn populate_fragments
@@ -89,6 +130,8 @@ fn gpu_array_fragment_extract
 
 #push-options "--debug SMTFail --split_queries always"
 #push-options "--print_implicits"
+#push-options "--print_full_names"
+
 inline_for_extraction noextract
 fn subproducts_tc_2d
   (#et_ab #et_acc : Type0)
@@ -135,9 +178,9 @@ fn subproducts_tc_2d
     invariant
       exists*
         (vdotIdx : sz{vdotIdx <= bk})
-        (emAFrags : erased (lseq (ematrix et_ab tm tk) wm))
-        (emBFrags : erased (lseq (ematrix et_ab tk tn) wn))
-        (emAccumFrags : erased (lseq (ematrix et_acc tm tn) (wm*wn))).
+        (emAFrags : lseq (ematrix et_ab tm tk) wm)
+        (emBFrags : lseq (ematrix et_ab tk tn) wn)
+        (emAccumFrags : lseq (ematrix et_acc tm tn) (wm*wn)).
           dotIdx |-> vdotIdx **
           array_fragment_pts_to aFrags emAFrags **
           array_fragment_pts_to bFrags emBFrags **
@@ -152,70 +195,76 @@ fn subproducts_tc_2d
       invariant
         exists*
           (vi : sz{vi <= wm})
-          (emAFrags : erased (lseq (ematrix et_ab tm tk) wm)).
+          (emAFrags : lseq (ematrix et_ab tm tk) wm).
             i0 |-> vi **
             array_fragment_pts_to aFrags emAFrags
     {
+      with emAFrags. assert array_fragment_pts_to aFrags emAFrags;
       // create tile for tensor core tiles that belong to the warp
-      let tile_for_tc_tiles = gpu_matrix_extract_tile_ro' gA (wm*tm) (SZ.v tk) (SZ.v arow) (SZ.v !dotIdx);
-      let a_tile = gpu_matrix_extract_tile_ro' tile_for_tc_tiles (SZ.v tm) (SZ.v tk) (SZ.v !i0) 0;
+      // let tile_for_tc_tiles = gpu_matrix_extract_tile_ro' gA (wm*tm) (SZ.v tk) (SZ.v arow) (SZ.v !dotIdx);
+      // let a_tile = gpu_matrix_extract_tile_ro' tile_for_tc_tiles (SZ.v tm) (SZ.v tk) (SZ.v !i0) 0;
       // Expected are only nats, but later on when the tile is used we need to concretize.
       // In this case wm*tm and 0 must be concretizable which means that either we have to write (SZ.v (wm*^tm)) and (SZ.v 0sz),
       // which is odd, because a nat is expected, or there must be type classes that can resolve this.
-      assert (rewrites_to a_tile (
-        gpu_matrix_subtile (
-          gpu_matrix_subtile gA (wm*tm) (SZ.v tk) (SZ.v arow) (SZ.v !dotIdx))
-          (SZ.v tm) (SZ.v tk) (SZ.v !i0) 0));
+      // assert (rewrites_to a_tile (
+      //   gpu_matrix_subtile (
+      //     gpu_matrix_subtile gA (wm*tm) (SZ.v tk) (SZ.v arow) (SZ.v !dotIdx))
+      //     (SZ.v tm) (SZ.v tk) (SZ.v !i0) 0));
 
-      unfold array_fragment_pts_to aFrags;
-      with saFrags. assert aFrags |-> saFrags;
+      assert pure (Seq.length emAFrags == wm);
+      let i0' = !i0;
+      assert pure (SZ.v i0' < Seq.length emAFrags);
+
+      array_fragment_extract #et_ab #FragA #tm #tn #tk #FragLRM aFrags emAFrags i0' ();
+      admit();
       let a_frag = aFrags.(!i0);
-      forevery_extract' #(natlt (Seq.length saFrags)) !i0 _;
+
+      let a_tile = 1;
 
       mma_loadA a_frag a_tile;
 
       // TODO purification does not seem to work under lambdas
       let vi = !i0;
       let vdotIdx = !dotIdx;
-      Pulse.Lib.Forall.elim_forall
-        // type annotation is required, although it is not required in the RefArray example
-        (fun (i : natlt (Seq.length saFrags)) ->
-            if i = (SZ.v vi)
-            then ((saFrags @! i) |-> (ematrix_subtile (ematrix_subtile eA (wm*tm) tk arow vdotIdx) tm tk vi 0))
-            else ((saFrags @! i) |-> (emAFrags @! i)));
+      // Pulse.Lib.Forall.elim_forall
+      //   // type annotation is required, although it is not required in the RefArray example
+      //   (fun (i : natlt (Seq.length saFrags)) ->
+      //       if i = (SZ.v vi)
+      //       then ((saFrags @! i) |-> (ematrix_subtile (ematrix_subtile eA (wm*tm) tk arow vdotIdx) tm tk vi 0))
+      //       else ((saFrags @! i) |-> (emAFrags @! i)));
 
-      assume 
-      pure (forall (x: natlt (Seq.Base.length saFrags) {~(x == SZ.v vi)}).
-        (match x = SZ.v vi with
-          | true ->
-            Seq.Base.index saFrags x |->
-            ematrix_subtile (ematrix_subtile eA
-                  (SZ.v wm * SZ.v tm)
-                  (SZ.v tk)
-                  (SZ.v arow)
-                  (SZ.v vdotIdx))
-              (SZ.v tm)
-              (SZ.v tk)
-              (SZ.v vi)
-              0
-          | _ -> Seq.Base.index saFrags x |-> Seq.Base.index emAFrags x) ==
-      fragment_pts_to (Seq.Base.index saFrags x) (Seq.Base.index emAFrags x));
+      // assume 
+      // pure (forall (x: natlt (Seq.Base.length saFrags) {~(x == SZ.v vi)}).
+      //   (match x = SZ.v vi with
+      //     | true ->
+      //       Seq.Base.index saFrags x |->
+      //       ematrix_subtile (ematrix_subtile eA
+      //             (SZ.v wm * SZ.v tm)
+      //             (SZ.v tk)
+      //             (SZ.v arow)
+      //             (SZ.v vdotIdx))
+      //         (SZ.v tm)
+      //         (SZ.v tk)
+      //         (SZ.v vi)
+      //         0
+      //     | _ -> Seq.Base.index saFrags x |-> Seq.Base.index emAFrags x) ==
+      // fragment_pts_to (Seq.Base.index saFrags x) (Seq.Base.index emAFrags x));
 
-      Pulse.Lib.Trade.elim_trade _ (forall+ (x: natlt (Seq.Base.length saFrags)).
-          match x = SZ.v vi with
-          | true ->
-            Seq.Base.index saFrags x |->
-            ematrix_subtile (ematrix_subtile eA
-                  (SZ.v wm * SZ.v tm)
-                  (SZ.v tk)
-                  (SZ.v arow)
-                  (SZ.v vdotIdx))
-              (SZ.v tm)
-              (SZ.v tk)
-              (SZ.v vi)
-              0
-          | _ -> Seq.Base.index saFrags x |-> Seq.Base.index emAFrags x);
-      admit();
+      // Pulse.Lib.Trade.elim_trade _ (forall+ (x: natlt (Seq.Base.length saFrags)).
+      //     match x = SZ.v vi with
+      //     | true ->
+      //       Seq.Base.index saFrags x |->
+      //       ematrix_subtile (ematrix_subtile eA
+      //             (SZ.v wm * SZ.v tm)
+      //             (SZ.v tk)
+      //             (SZ.v arow)
+      //             (SZ.v vdotIdx))
+      //         (SZ.v tm)
+      //         (SZ.v tk)
+      //         (SZ.v vi)
+      //         0
+      //     | _ -> Seq.Base.index saFrags x |-> Seq.Base.index emAFrags x);
+      // admit();
 
 
 
